theories/compiler/linear_imp.v
@@ -57,11 +57,13 @@ Proof. elim: e => //= *; rewrite ?andb_True; split!; apply lexpr_op_is_static. Q
 
 Record lfndef : Type := {
   lfd_args : list string;
+  lfd_vars : list (string * Z);
   lfd_body : lexpr;
 }.
 
 Program Definition lfndef_to_fndef (fn : lfndef) : fndef := {|
    fd_args := fn.(lfd_args);
+   fd_vars := fn.(lfd_vars);
    fd_body := lexpr_to_expr fn.(lfd_body);
 |}.
 Next Obligation. move => ?. apply lexpr_is_static. Qed.
