theories/compiler/monad.v
@@ -1,4 +1,5 @@
 Require Import refframe.base.
+Require Import refframe.axioms.
 
 Set Default Proof Using "Type".
 
@@ -145,6 +146,13 @@ Section compiler_monad.
     rewrite /crun/mbind/cbind/=.
     repeat case_match; simplify_eq/= => //.
     by rewrite assoc_L.
+  Qed.
+
+  Lemma cmap_S {B C} xs f n:
+    cmap xs n f = cmap (A:=A) (S:=S) (B:=B) (C:=C) (E:=E) xs (Datatypes.S n) (f ∘ pred).
+  Proof.
+    elim: xs n f => //= ?? IH n f.
+    f_equal. apply functional_extensionality => ?. by rewrite IH.
   Qed.
 
   Lemma cret_success R (r' : R) (s s' : S) (a : A) (r : R):
